compiler/inference/unify_cvScript.sml
@@ -13,11 +13,9 @@ Theorem tcvwalk_pre:
   ∀s t. cwfs s ⇒ tcvwalk_pre s t
 Proof
   rpt strip_tac >> drule_then assume_tac $ SRULE[FORALL_PROD]WF_cvwalkR >>
-  ‘∀p. FST p = s ⇒ (λ(s0,n). tcvwalk_pre s0 n) p’
-    suffices_by simp[FORALL_PROD] >>
+  ‘∀t. tcvwalk_pre s t’ suffices_by simp[] >>
   IMP_RES_THEN ho_match_mp_tac relationTheory.WF_INDUCTION_THM >>
-  simp[FORALL_PROD] >> qx_gen_tac ‘n’ >>
-  strip_tac >>
+  qx_gen_tac ‘n’ >> strip_tac >>
   simp[Once tcvwalk_pre_def] >> rw[] >>
   drule (SRULE[FORALL_PROD]cvwalk_ensures_decrease) >>
   simp[cvwalk_code_def, AllCaseEqs()]
@@ -36,11 +34,10 @@ val tcocwl_pre_def = cv_trans_pre tcocwl_thm;
 Theorem tcocwl_pre:
   ∀s n wl. cwfs s ⇒ tcocwl_pre s n wl
 Proof
-  rpt strip_tac >> drule_then assume_tac WF_kcocwlR >>
-  ‘∀t. FST t = s ⇒ (λ(s,n,wl). tcocwl_pre s n wl) t’
-    suffices_by simp[FORALL_PROD] >>
+  rpt strip_tac >> drule_then (qspec_then ‘n’ assume_tac) WF_kcocwlR >>
+  ‘∀wl. tcocwl_pre s n wl’ suffices_by simp[] >>
   IMP_RES_THEN ho_match_mp_tac relationTheory.WF_INDUCTION_THM >>
-  simp[FORALL_PROD] >> qx_genl_tac [‘n’, ‘wl’] >> strip_tac >>
+  simp[] >> qx_gen_tac ‘wl’ >> strip_tac >>
   simp[Once tcocwl_pre_def] >> rw[] >> simp[tcwalk_pre] >>
   drule (SRULE[FORALL_PROD]kcocwl_ensures_decrease) >>
   simp[kcocwl_code_def]
@@ -48,17 +45,37 @@ QED
 
 val tcunify_pre_def = cv_trans_pre tcunify_thm;
 
+Theorem tcunify_pre_thm:
+  cwfs s ⇒
+  (tcunify_pre s wl ⇔
+     ∀s' wl'. cunify_code (s,wl) = INL (s',wl') ⇒ tcunify_pre s' wl')
+Proof
+  strip_tac >> simp[SimpLHS, Once tcunify_pre_def] >>
+  simp[cunify_code_def, AllCaseEqs(), PULL_EXISTS] >>
+  iff_tac >> rw[] >> gvs[tcwalk_pre, tcocwl_pre]
+QED
+
+Theorem tcunify_pre:
+  ∀s wl. cwfs s ⇒ tcunify_pre s wl
+Proof
+  assume_tac WF_kcunifywlR >>
+  ‘∀p. cwfs (FST p) ⇒ tcunify_pre (FST p) (SND p)’
+    suffices_by simp[FORALL_PROD] >>
+  IMP_RES_THEN ho_match_mp_tac relationTheory.WF_INDUCTION_THM >>
+  simp[FORALL_PROD] >> rpt strip_tac >> rename [‘(s,wl)’] >>
+  simp[Once tcunify_pre_thm] >> rpt strip_tac >>
+  first_x_assum irule >>
+  simp[kcunifywl_ensures_decrease] >>
+  irule (SRULE[FORALL_PROD]kcunifywl_preserves_precond) >>
+  metis_tac[]
+QED
+
 val cunify_pre_def = cv_trans_pre tcunify_correct;
 
 Theorem cunify_pre[cv_pre]:
   cunify_pre s t1 t2 ⇔ cwfs s
 Proof
-  qsuff_tac ‘cwfs s ⇒ cunify_pre s t1 t2’
-  >- metis_tac [cunify_pre_def]
-  \\ gvs [cunify_pre_def]
-  \\ simp[Once tcunify_pre_def]
-  \\ rpt strip_tac
-  \\ cheat
+  simp[EQ_IMP_THM, cunify_pre_def, tcunify_pre]
 QED
 
 val _ = export_theory ();
